WIP; spinlock all

examples/spinlock/SpinLockAll.v
@@ -7,28 +7,108 @@ Require Import ElimRel SModCancel Cancellation.
 
 Module IncrAll.
   Import inv_instances.
-  Local Instance Γ : HRA := ##[invΓ; memΓ; SpinLockΓ; SpinLockMainAΓ].
+  Local Instance Γ : HRA := ##[invΓ; memΓ; SchAΓ; SpinLockΓ; SpinLockMainAΓ].
   Local Instance Σ : GRA := ##[invΣ; SchAΣ; Γ].
 
-  Local Definition spc_user_s : univ_id → string → option fspec :=
-    λ u, to_spc (SpinLockMainAS.spc u ++ MemA.Spc).
-
-  Local Definition smod_src : univ_id → SMod.t :=
-    λ u, (SpinLockMainA.Mod u) ☆ (MemA.Mod) ☆ (SchA.Mod u (spc_user_s u)).
-  Local Definition spc_s : univ_id → string → option fspec :=
-    λ u, spc_from (smod_src u).
-
-  Local Definition smod_cancel : univ_id → HMod.t :=
-    λ u, SModCancel.to_hmod (smod_src u).
-
-  Local Definition mod_src : univ_id → HMod.t :=
-    λ u, SMod.to_hmod (wsim_ginv u ⊤) (spc_s u) (smod_src u).
-
+  (* building the target module *)
   Local Definition csl : string → bool := λ _, false.
   Local Definition genv : GEnv.t := GEnv.unit.
-(* 
-  Local Definition mod_tgt : HMod.t := SpinLockMainI.t ★ (MemI.t csl genv) ★ (SchI.t).
+  Local Definition mod_tgt : HMod.t := SpinLockMainI.t ★ MemI.t csl genv ★ SchI.t ★ SpinLockI.t.
 
+  (* building the source module *)
+  Local Definition u : univ_id := 1.
+
+  Local Definition spc_user_s : string → option fspec :=
+    to_spc (SpinLockMainAS.spc u ++ MemA.Spc ++ SpinLockAS.spc u).
+
+  Local Definition smod_src : SMod.t :=
+    SpinLockMainA.Mod u ☆ MemA.Mod ☆ SchA.Mod u spc_user_s ☆ SpinLockA.Mod u.
+  Local Definition spc_s : string → option fspec :=
+    spc_from smod_src.
+  Local Definition mod_src : HMod.t := SMod.to_hmod (wsim_ginv u ⊤) spc_s smod_src.
+  Local Definition init_cond : iProp Σ := (MemA.InitCond csl genv ∗ SchA.InitCond)%I.
+
+  (* source module after cancellation *)
+  Local Definition smod_cancel : HMod.t := SModCancel.to_hmod smod_src.
+
+  (* Refinement between smod_cancel and smod_src *)
+  Local Definition main_fsp : fspec := SpinLockMainAS.main_spec u.
+  Lemma cancel_src :
+    refines (smod_cancel, init_cond ∗ main_fsp.(precond) tt tt↑ tt↑)%I
+            (mod_src,     init_cond).
+  Proof. eapply cancellation; try by econs. i. unfold_pre_post. iIntros "[_ [-> ->]]". done. Qed.
+
+  (* Refinement between smod_src and mod_tgt *)
+  Lemma src_tgt : refines (mod_src, init_cond) (mod_tgt, emp%I).
+  Proof.
+    apply ctxr_refines.
+    rewrite /mod_src /smod_src /mod_tgt /init_cond ?add_interp_comm.
+    etrans.
+    { do 2 eapply ctxr_frameL. eapply ctxr_comm. }
+    do 2 rewrite -hmod_add_assoc.
+    etrans.
+    { eapply ctxr_frameR.
+      replace (SMod.to_hmod _ _ (SpinLockMainA.Mod _)) with (SpinLockMainA.t u spc_s); cycle 1.
+      { unfold_hmod; ss. }
+      replace (SMod.to_hmod _ _ (MemA.Mod)) with (MemA.t u spc_s); cycle 1.
+      { unfold_hmod; ss. }
+      replace (SMod.to_hmod _ _ (SpinLockA.Mod _)) with (SpinLockA.t u spc_s); cycle 1.
+      { unfold_hmod; ss. }
+      rewrite hmod_add_assoc -hmod_addc_empty_l.
+      etrans; first eapply ctxr_cond_frameR.
+      { eapply SpinLockMainIA.wctxr; eauto.
+        { instantiate (1:=spc_user_s).
+          rewrite /spc_user_s /SchAS.spc /spc_s /smod_src; unseal CRIS. split; first prove_nodup.
+          ii. ss; des_ifs; rewrite ->eq_rel_dec_correct in *; des_ifs.
+        }
+        { rewrite /spc_user_s /SchAS.spc /spc_s /smod_src; unseal CRIS. split; first prove_nodup.
+          ii. ss; des_ifs; rewrite ->eq_rel_dec_correct in *; des_ifs.
+        }
+        { rewrite /spc_user_s /MemA.Spc /spc_s /smod_src; unseal CRIS. split; first prove_nodup.
+          ii. ss; des_ifs; rewrite ->eq_rel_dec_correct in *; des_ifs.
+        }
+      }
+      rewrite hmod_addc_empty_l. refl.
+    }
+    rewrite hmod_add_assoc. eapply ctxr_frameL.
+    etrans.
+    { eapply ctxr_frameR. rewrite -hmod_addc_empty_l. eapply ctxr_cond_frameR.
+      etrans; first eapply ctxr_comm.
+      eapply SpinLockIA.wctxr.
+      { rewrite /spc_user_s /SchAS.spc /spc_s /smod_src; unseal CRIS. split; first prove_nodup.
+        ii. ss; des_ifs; rewrite ->eq_rel_dec_correct in *; des_ifs.
+      }
+      { rewrite /spc_user_s /spc_s /smod_src /MemA.Spc; unseal CRIS. split; first prove_nodup.
+        ii. ss; des_ifs; rewrite ->eq_rel_dec_correct in *; des_ifs.
+      }
+    }
+    rewrite hmod_add_assoc.
+    etrans; first eapply ctxr_comm. rewrite -hmod_add_assoc. eapply ctxr_frameR.
+    etrans.
+    { rewrite hmod_addc_empty_l. eapply ctxr_frameR, ctxr_cond_frameR. eapply MemIA.correct.
+      rewrite /MemA.Spc; unseal CRIS.
+      split; first prove_nodup. ii; ss; des_ifs; rewrite ->eq_rel_dec_correct in *; des_ifs.
+    }
+    eapply ctxr_frameL.
+    etrans.
+    { replace (SMod.to_hmod _ _ (SchA.Mod _ _)) with (SchA.t u spc_s spc_user_s); cycle 1.
+      { unfold_hmod; ss. }
+      rewrite hmod_addc_empty_l.
+      eapply SchIA.wctxr.
+      { rewrite /spc_user_s /SchAS.spc /spc_s /smod_src; unseal CRIS. split; first prove_nodup.
+        ii. ss; des_ifs; rewrite ->eq_rel_dec_correct in *; des_ifs.
+      }
+      { rewrite /spc_user_s /SchAS.spc /spc_s /smod_src /MemA.Spc; unseal CRIS.
+        ii. ss; des_ifs; rewrite ->eq_rel_dec_correct in *; des_ifs.
+      }
+    }
+    refl.
+  Qed.
+
+  Local Definition initial_resource : Σ :=
+    own_admin MainAS.init_res ⋅ CannonAS.init_res.
+
+(* 
   Local Definition SchInSpc : ∀ u, spc_incl (SchAS.spc u (spc_user_s u)) (spc_s u).
   Proof.
     ii; rewrite /spc_s /SchAS.spc /MemA.Spc /IncrMainAS.spc; unseal CRIS; split; [prove_nodup|ii].
