examples/spinlock/SpinLockMainIAProof.v
@@ -78,59 +78,59 @@ Module SpinLockMainIA. Section SpinLockMainIA.
   Lemma main_simF : HSim.sim_fun open MA MI IstFull SpinLockMainName.main.
   Proof.
     winit_simF u_a 0.
-    wsteps_l. iDestruct "ASM" as "[-> ->]". hss.
-    wsteps_r. sch_yield_r. iSplitL "IST"; ss; clear nths; iIntros (nths st_s st_t) "IST".
+    wsteps_l. iDestruct "ASM" as "[[-> TID] ->]". hss.
+    wsteps_r. sch_yield_r. iFrame; ss; clear nths; iIntros (nths st_s st_t) "IST TID".
     winline_r. wforce_r 1. wforces_r. iSplit; eauto.
     wsteps_r. iDestruct "GRT" as "[[%blk [-> [GRT _]]] ->]". hss. wsteps_r.
-    wsteps_r. sch_yield_r. iSplitL "IST"; ss; clear nths st_s st_t; iIntros (nths st_s st_t) "IST".
+    wsteps_r. sch_yield_r. iFrame; ss; clear nths st_s st_t; iIntros (nths st_s st_t) "IST TID".
     winline_r. wforce_r (blk, 0%Z, Vint 0). wforces_r. iFrame; iSplit; eauto.
     wsteps_r. iDestruct "GRT" as "[[PT ->] ->]". hss. wsteps_r.
-    wsteps_r. sch_yield_r. iSplitL "IST"; ss; clear nths st_s st_t; iIntros (nths st_s st_t) "IST".
+    wsteps_r. sch_yield_r. iFrame; ss; clear nths st_s st_t; iIntros (nths st_s st_t) "IST TID".
     (* create lock-guarded proposition *)
     iApply (wsim_own_alloc (●F 0%Z ⋅ ◯F{1} 0%Z)).
     { eapply frac_auth_valid; ss. }
     iIntros "[%γ [B W]]".
-    winline_r. wforce_r (existT 0 (lock_P (blk, 0%Z) γ)). wforces_r. iSplitL "B PT"; eauto.
-    { SL_red; iSplit; eauto. iExists _; SL_red; iFrame. }
+    winline_r. wforce_r (0, existT 0 (lock_P (blk, 0%Z) γ)). wforces_r. iSplitL "TID B PT"; eauto.
+    { SL_red; iSplit; eauto. iFrame. iExists _; SL_red; iFrame. }
     wsteps_r. hss. wsteps_r.
-    sch_yield_r. iSplitL "IST"; ss; clear nths st_s st_t; iIntros (nths st_s st_t) "IST".
-    wsteps_r. iDestruct "GRT" as "[[%val [%γ_l [-> #I]]] %EQ]". hss. wsteps_r.
-    sch_yield_r. iSplitL "IST"; ss; clear nths st_s st_t; iIntros (nths st_s st_t) "IST".
+    sch_yield_r. iFrame; ss; clear nths st_s st_t; iIntros (nths st_s st_t) "IST".
+    wsteps_r. iDestruct "GRT" as "[[TID [%val [%γ_l [-> #I]]]] %EQ]". hss. wsteps_r.
+    sch_yield_r. iFrame; ss; clear nths st_s st_t; iIntros (nths st_s st_t) "IST TID".
     iPoseProof "I" as "[%b_l [%o_l [-> _]]]".
     sch_yield_l. wsteps_l. wforce_l (Vptr b_l o_l, Vptr blk 0). wsteps_l. sch_yield_l.
     (* create preconditions of incr *)
     iDestruct "W" as "[W1 W2]".
     wsteps_l. sch_spawn.
     { apply MainInSpc; ss. }
-    { eapply (incr_spawnable u_a). }
-    iSplitL "IST"; ss; clear nths st_s st_t.
-    iSplitL "W1".
-    { rewrite /incr_pre. iExists _. iFrame. done. }
-    iIntros (tid nths st_s st_t) "IST TKN".
+    { eapply (incr_spawnable). }
+    iFrame; ss; clear nths st_s st_t.
+    iSplit.
+    { iSplit; eauto. }
+    iIntros (tid nths st_s st_t) "IST TID TKN".
     wsteps_l. wsteps_r.
-    sch_yield_r. iSplitL "IST"; ss; clear nths st_s st_t; iIntros (nths st_s st_t) "IST".
+    sch_yield_r. iFrame; ss; clear nths st_s st_t; iIntros (nths st_s st_t) "IST TID".
     sch_yield_l. wsteps_l.
     sch_spawn.
     { apply MainInSpc; ss. }
     { eapply (incr_spawnable u_a). }
-    iSplitL "IST"; ss; clear nths st_s st_t.
-    iSplitL "W2".
-    { rewrite /incr_pre. iExists _. iFrame. done. }
-    iIntros (tid2 nths st_s st_t) "IST TKN2".
+    iSplitL "IST"; ss; clear nths st_s st_t. iFrame.
+    iSplit.
+    { iSplit; eauto. }
+    iIntros (tid2 nths st_s st_t) "IST TID TKN2".
     wsteps_l. wsteps_r.
-    sch_yield_r. iSplitL "IST"; ss; clear nths st_s st_t; iIntros (nths st_s st_t) "IST".
+    sch_yield_r. iFrame; ss; clear nths st_s st_t; iIntros (nths st_s st_t) "IST TID".
     sch_yield_l. wsteps_l.
     sch_join; iFrame.
-    clear nths st_s st_t; iIntros (nths st_s st_t ret) "IST W1 /=".
-    wsteps_r. sch_yield_r. iSplitL "IST"; ss; clear nths st_s st_t; iIntros (nths st_s st_t) "IST".
+    clear nths st_s st_t; iIntros (nths st_s st_t ret) "IST TID W1 /=".
+    wsteps_r. sch_yield_r. iFrame; ss; clear nths st_s st_t; iIntros (nths st_s st_t) "IST TID".
     sch_yield_l. wsteps_l.
     sch_join; iFrame.
-    clear nths st_s st_t; iIntros (nths st_s st_t ret2) "IST W2 /=".
+    clear nths st_s st_t; iIntros (nths st_s st_t ret2) "IST TID W2 /=".
     wsteps_l. wsteps_r.
     unfold_iter_l. wsteps_l.
-    sch_yield_r. iSplitL "IST"; ss; clear nths st_s st_t; iIntros (nths st_s st_t) "IST".
+    sch_yield_r. iFrame; ss; clear nths st_s st_t; iIntros (nths st_s st_t) "IST TID".
     sch_yield_l. wforce_l false. wsteps_l.
-    winline_r. wforce_r (γ_l, Vptr b_l o_l, existT 0 (lock_P (blk, 0%Z) γ)). wforces_r.
+    winline_r. wforce_r (0, γ_l, Vptr b_l o_l, existT 0 (lock_P (blk, 0%Z) γ)). wforces_r. iFrame.
     iSplit; eauto.
     wsteps_r. hss. wsteps_r.
     (* lock acquire coinduction *)
@@ -141,25 +141,25 @@ Module SpinLockMainIA. Section SpinLockMainIA.
     sch_yield_r. iSplitL "IST"; ss; clear nths st_s st_t; iIntros (nths st_s st_t) "IST".
     wsteps_r. destruct q; cycle 1.
     { wsteps_r. sch_yield_l. wforce_l false. wsteps_l. wby_coind "CIH". iFrame. ss. }
-    wsteps_r. iDestruct "GRT" as "[[-> [TKN P]] _]". hss. wsteps_r.
+    wsteps_r. iDestruct "GRT" as "[[-> [TID [TKN P]]] _]". hss. wsteps_r.
     SL_red. iCombine "W1 W2" as "W". iDestruct "P" as "[%x P]"; SL_red; iDestruct "P" as "[PT B]".
     iCombine "B W" gives %WF%frac_auth_agree. inv WF.
-    sch_yield_r. iSplitL "IST"; ss; clear nths st_s st_t; iIntros (nths st_s st_t) "IST".
+    sch_yield_r. iFrame; ss; clear nths st_s st_t; iIntros (nths st_s st_t) "IST TID".
     winline_r. wforce_r (blk, 0%Z, Vint 2%Z, 1%Qp). wforces_r. iSplitL "PT"; eauto.
     wsteps_r. iDestruct "GRT" as "[[PT ->] ->]". hss. wsteps_r.
-    sch_yield_r. iSplitL "IST"; ss; clear nths st_s st_t; iIntros (nths st_s st_t) "IST". wsteps_r.
-    sch_yield_r. iSplitL "IST"; ss; clear nths st_s st_t; iIntros (nths st_s st_t) "IST".
-    winline_r. wforce_r (γ_l, Vptr b_l o_l, existT 0 (lock_P (blk, 0%Z) γ)). wforces_r.
-    iSplitL "TKN B PT".
+    sch_yield_r. iFrame; ss; clear nths st_s st_t; iIntros (nths st_s st_t) "IST TID". wsteps_r.
+    sch_yield_r. iFrame; ss; clear nths st_s st_t; iIntros (nths st_s st_t) "IST TID".
+    winline_r. wforce_r (0, γ_l, Vptr b_l o_l, existT 0 (lock_P (blk, 0%Z) γ)). wforces_r.
+    iSplitL "TKN TID B PT".
     { SL_red. iSplit; eauto. iFrame. iSplit; eauto. iSplit; eauto. iExists _; SL_red; iFrame. }
     wsteps_r. hss. wsteps_r.
-    sch_yield_r. iSplitL "IST"; ss; clear nths st_s st_t; iIntros (nths st_s st_t) "IST".
-    wsteps_r. iDestruct "GRT" as "[-> _]". hss. wsteps_r.
-    sch_yield_r. iSplitL "IST"; ss; clear nths st_s st_t; iIntros (nths st_s st_t) "IST".
+    sch_yield_r. iFrame; ss; clear nths st_s st_t; iIntros (nths st_s st_t) "IST".
+    wsteps_r. iDestruct "GRT" as "[[-> TID] _]". hss. wsteps_r.
+    sch_yield_r. iFrame; ss; clear nths st_s st_t; iIntros (nths st_s st_t) "IST TID".
     sch_yield_l. wforce_l true. wsteps_l.
     sch_yield_l. wstep.
     wsteps_l. wsteps_r.
-    sch_yield_r. iSplitL "IST"; ss; clear nths st_s st_t; iIntros (nths st_s st_t) "IST". wsteps_r.
+    sch_yield_r. iFrame; ss; clear nths st_s st_t; iIntros (nths st_s st_t) "IST TID". wsteps_r.
     sch_yield_l. wsteps_l. wforces_l. iSplit; eauto. wsteps_l. wstep.
     iSplit; eauto.
   Qed.
@@ -174,14 +174,14 @@ Module SpinLockMainIA. Section SpinLockMainIA.
 End SpinLockMainIA.
 Section wctxr.
   Context `{!invG α Σ Γ, !subG Γ Σ, !sinvG Σ Γ α β τ}.
-  Context `{!SchAGΣ Σ, !memGΓ Γ, !SpinLockMainAGΓ Γ, !SpinLockAGΓ Γ}.
+  Context `{!SchAGΣ Σ, !SchAGΓ Γ, !memGΓ Γ, !SpinLockMainAGΓ Γ, !SpinLockAGΓ Γ}.
 
-  Definition wctxr (u : univ_id) (spc_s spc_user_s spc_mem : univ_id → string → option fspec)
-      (SchInSpc : ∀ u, spc_incl (SchAS.spc u (spc_user_s u)) (spc_s u))
-      (MainInSpc : ∀ u, spc_incl (SpinLockMainAS.spc u) (spc_user_s u))
-      (MemInSpc : ∀ u, spc_incl MemA.Spc (spc_s u)) :
+  Definition wctxr (u : univ_id) (spc_s spc_user_s spc_mem : string → option fspec)
+      (SchInSpc : spc_incl (SchAS.spc u spc_user_s) spc_s)
+      (MainInSpc : spc_incl (SpinLockMainAS.spc u) spc_user_s)
+      (MemInSpc : spc_incl MemA.Spc spc_s) :
     ctx_refines
-      ((SpinLockMainA.t u (spc_s u)) ★ (MemA.t u (spc_mem u) ★ (SpinLockA.t u (spc_s u))), emp%I)
-      ((SpinLockMainI.t)             ★ (MemA.t u (spc_mem u) ★ (SpinLockA.t u (spc_s u))), emp%I).
+      ((SpinLockMainA.t u spc_s) ★ (MemA.t u spc_mem ★ (SpinLockA.t u spc_s)), emp%I)
+      ((SpinLockMainI.t)         ★ (MemA.t u spc_mem ★ (SpinLockA.t u spc_s)), emp%I).
   Proof. eapply main_adequacy, sim; eauto. Qed.
 End wctxr. End SpinLockMainIA.
